libcrux-ml-kem/src/vector/avx2/arithmetic.rs
@@ -22,13 +22,7 @@ pub(crate) fn sub(lhs: Vec256, rhs: Vec256) -> Vec256 {
 pub(crate) fn multiply_by_constant(vector: Vec256, constant: i16) -> Vec256 {
     let cv = mm256_set1_epi16(constant);
     let result = mm256_mullo_epi16(vector, cv);
-    hax_lib::fstar!("Spec.Utils.lemma_map2_index #_ #_ #_ #(sz 16) mul_mod 
-                        (Libcrux_intrinsics.Avx2_extract.vec256_as_i16x16 ${vector})
-                        (Libcrux_intrinsics.Avx2_extract.vec256_as_i16x16 ${cv});
-                     Spec.Utils.lemma_map_index #_ #_ #(sz 16) (fun x -> x *. constant) 
-                        (Libcrux_intrinsics.Avx2_extract.vec256_as_i16x16 ${vector});
-                     Spec.Utils.lemma_create_index #_ (sz 16) constant;
-                     Seq.lemma_eq_intro (Libcrux_intrinsics.Avx2_extract.vec256_as_i16x16 ${result})
+    hax_lib::fstar!("Seq.lemma_eq_intro (Libcrux_intrinsics.Avx2_extract.vec256_as_i16x16 ${result})
                         (Spec.Utils.map_array (fun x -> x *. $constant) (Libcrux_intrinsics.Avx2_extract.vec256_as_i16x16 $vector))");
     
     result
@@ -40,13 +34,7 @@ pub(crate) fn multiply_by_constant(vector: Vec256, constant: i16) -> Vec256 {
 pub(crate) fn bitwise_and_with_constant(vector: Vec256, constant: i16) -> Vec256 {
     let cv = mm256_set1_epi16(constant);
     let result = mm256_and_si256(vector, cv);
-    hax_lib::fstar!("Spec.Utils.lemma_map2_index #_ #_ #_ #(sz 16) (&.) 
-                        (Libcrux_intrinsics.Avx2_extract.vec256_as_i16x16 ${vector})
-                        (Libcrux_intrinsics.Avx2_extract.vec256_as_i16x16 ${cv});
-                     Spec.Utils.lemma_map_index #_ #_ #(sz 16) (fun x -> x &. constant) 
-                        (Libcrux_intrinsics.Avx2_extract.vec256_as_i16x16 ${vector});
-                     Spec.Utils.lemma_create_index #_ (sz 16) constant;
-                     Seq.lemma_eq_intro (Libcrux_intrinsics.Avx2_extract.vec256_as_i16x16 ${result})
+    hax_lib::fstar!("Seq.lemma_eq_intro (Libcrux_intrinsics.Avx2_extract.vec256_as_i16x16 ${result})
                         (Spec.Utils.map_array (fun x -> x &. $constant) (Libcrux_intrinsics.Avx2_extract.vec256_as_i16x16 $vector))");
     result
 }
@@ -58,9 +46,7 @@ pub(crate) fn bitwise_and_with_constant(vector: Vec256, constant: i16) -> Vec256
                             Spec.Utils.map_array (fun x -> x >>! ${SHIFT_BY}) (Libcrux_intrinsics.Avx2_extract.vec256_as_i16x16 $vector)"))]   
 pub(crate) fn shift_right<const SHIFT_BY: i32>(vector: Vec256) -> Vec256 {
     let result = mm256_srai_epi16::<{ SHIFT_BY }>(vector);
-    hax_lib::fstar!("Spec.Utils.lemma_map_index #_ #_ #(sz 16) (fun x -> x >>! ${SHIFT_BY}) 
-                        (Libcrux_intrinsics.Avx2_extract.vec256_as_i16x16 ${vector});
-                     Seq.lemma_eq_intro (Libcrux_intrinsics.Avx2_extract.vec256_as_i16x16 ${result})
+    hax_lib::fstar!("Seq.lemma_eq_intro (Libcrux_intrinsics.Avx2_extract.vec256_as_i16x16 ${result})
                         (Spec.Utils.map_array (fun x -> x >>! ${SHIFT_BY}) 
                            (Libcrux_intrinsics.Avx2_extract.vec256_as_i16x16 $vector))");
     result
@@ -78,30 +64,18 @@ pub(crate) fn shift_right<const SHIFT_BY: i32>(vector: Vec256) -> Vec256 {
         Spec.Utils.map_array (fun x -> if x >=. 3329s then x -! 3329s else x) (Libcrux_intrinsics.Avx2_extract.vec256_as_i16x16 $vector)"))]   
 pub(crate) fn cond_subtract_3329(vector: Vec256) -> Vec256 {
     let field_modulus = mm256_set1_epi16(FIELD_MODULUS);
-    hax_lib::fstar!("Spec.Utils.lemma_create_index #_ (sz 16) ${FIELD_MODULUS}");
-
+    
     // Compute v_i - Q and crate a mask from the sign bit of each of these
     // quantities.
     let v_minus_field_modulus = mm256_sub_epi16(vector, field_modulus);
-    hax_lib::fstar!("Spec.Utils.lemma_map2_index #_ #_ #_ #(sz 16) (-.) 
-            (Libcrux_intrinsics.Avx2_extract.vec256_as_i16x16 $vector)
-            (Libcrux_intrinsics.Avx2_extract.vec256_as_i16x16 $field_modulus)");
-
+    
     let sign_mask = mm256_srai_epi16::<15>(v_minus_field_modulus);
-    hax_lib::fstar!("Spec.Utils.lemma_map_index #_ #_ #(sz 16) (fun x -> x >>! 15l) 
-            (Libcrux_intrinsics.Avx2_extract.vec256_as_i16x16 $v_minus_field_modulus)");
-
+    
     // If v_i - Q < 0 then add back Q to (v_i - Q).
     let conditional_add_field_modulus = mm256_and_si256(sign_mask, field_modulus);
-    hax_lib::fstar!("Spec.Utils.lemma_map2_index #_ #_ #_ #(sz 16) (&.) 
-            (Libcrux_intrinsics.Avx2_extract.vec256_as_i16x16 $sign_mask)
-            (Libcrux_intrinsics.Avx2_extract.vec256_as_i16x16 $field_modulus)");
-
+    
     let result = mm256_add_epi16(v_minus_field_modulus, conditional_add_field_modulus);
-    hax_lib::fstar!("Spec.Utils.lemma_map2_index #_ #_ #_ #(sz 16) (+.) 
-            (Libcrux_intrinsics.Avx2_extract.vec256_as_i16x16 $v_minus_field_modulus)
-            (Libcrux_intrinsics.Avx2_extract.vec256_as_i16x16 $conditional_add_field_modulus)");
-
+    
     result
 }
 
