libcrux-ml-kem/proofs/fstar/spec/Spec.Utils.fst
@@ -23,22 +23,31 @@ let create len c = createi len (fun i -> c)
 
 let repeati #acc (l:usize) (f:(i:usize{v i < v l}) -> acc -> acc) acc0 : acc = Lib.LoopCombinators.repeati (v l) (fun i acc -> f (sz i) acc) acc0
 
-let lemma_createi_index #a len f:
-  Lemma (forall i. Seq.index (createi #a len f) i == f (sz i)) = admit ()
+val lemma_createi_index #a len f i :
+  Lemma (Seq.index (createi #a len f) i == f (sz i))
+        [SMTPat (Seq.index (createi #a len f) i)]
+let lemma_createi_index #a len f i = ()
 
-let lemma_create_index #a len c:
-  Lemma (forall i. Seq.index (create #a len c) i == c) = admit ()
+val lemma_create_index #a len c i:
+  Lemma (Seq.index (create #a len c) i == c)
+        [SMTPat (Seq.index (create #a len c) i)]
+let lemma_create_index #a len c i = ()
 
-let lemma_map_index #a #b #len f x:
-  Lemma (forall i. Seq.index (map_array #a #b #len f x) i == f (Seq.index x i)) = admit ()
+val lemma_map_index #a #b #len f x i:
+  Lemma (Seq.index (map_array #a #b #len f x) i == f (Seq.index x i))
+        [SMTPat (Seq.index (map_array #a #b #len f x) i)]
+let lemma_map_index #a #b #len f x i = ()
 
-let lemma_map2_index #a #b #c #len f x y :
-  Lemma (forall i. Seq.index (map2 #a #b #c #len f x y) i == f (Seq.index x i) (Seq.index y i)) = admit ()
-
+val lemma_map2_index #a #b #c #len f x y i:
+  Lemma (Seq.index (map2 #a #b #c #len f x y) i == f (Seq.index x i) (Seq.index y i))
+        [SMTPat (Seq.index (map2 #a #b #c #len f x y) i)]
+let lemma_map2_index #a #b #c #len f x y i = ()
+  
 let lemma_bitand_properties #t (x:int_t t) :
-  Lemma ((x &. ones) == x /\ (x &. mk_int #t 0) == mk_int #t 0 /\ (ones #t &. x) == x /\ (mk_int #t 0 &. x) == mk_int #t 0) = admit()
+  Lemma ((x &. ones) == x /\ (x &. mk_int #t 0) == mk_int #t 0 /\ (ones #t &. x) == x /\ (mk_int #t 0 &. x) == mk_int #t 0) = 
+    logand_lemma #t x x
 
-#push-options "--fuel 0 --ifuel 0 --z3rlimit 500"
+#push-options "--z3rlimit 200"
 let flatten #t #n
   (#m: usize {range (v n * v m) usize_inttype})
   (x: t_Array (t_Array t m) n)
@@ -88,7 +97,8 @@ let update_at_range_lemma #n
     introduce forall (i:nat {i < len}). Seq.index s i == Seq.index s' i
     with (assert ( Seq.index (Seq.slice s  0 len) i == Seq.index s  i 
                  /\ Seq.index (Seq.slice s' 0 len) i == Seq.index s' i ))  
- 
+
+
 /// Bounded integers
 
 let is_i16b (l:nat) (x:i16) = (v x <= l) && (v x >= -l)
@@ -136,14 +146,24 @@ let mont_red_i32 (x:i32) : i16 =
   let vhigh = cast (x >>! 16l) <: i16 in
   vhigh -. k_times_modulus
 
-#push-options "--z3rlimit 900 --split_queries always"
+let lemma_at_percent_mod (v:int) (p:int{p>0/\ p%2=0}):
+  Lemma ((v @% p) % p == v % p) = ()
+
+let lemma_div_at_percent (v:int) (p:int{p>0/\ p%2=0 /\ (v/p) < p/2 /\ (v/p) >= -p / 2}):
+  Lemma ((v / p) @% p == v / p) = 
+    assert ((v / p) < p);
+    assert ((v / p) @% p == v / p);
+    ()
+
+#push-options "--z3rlimit 1200 --split_queries always"
 val lemma_mont_red_i32 (x:i32): Lemma
-  (requires (Spec.Utils.is_i32b (3328 * pow2 16) x))
+  (requires (is_i32b (3328 * pow2 16) x))
   (ensures (
           let result:i16 = mont_red_i32 x in
-          Spec.Utils.is_i16b (3328 + 1665) result /\
-          (Spec.Utils.is_i32b (3328 * 3328) x ==> Spec.Utils.is_i16b 3328 result) /\
+          is_i16b (3328 + 1665) result /\
+          (is_i32b (3328 * 3328) x ==> is_i16b 3328 result) /\
           v result % 3329 == (v x * 169) % 3329))
+          
 let lemma_mont_red_i32 (x:i32) =
   let vlow = cast x <: i16 in
   assert (v vlow == v x @% pow2 16);
@@ -158,28 +178,36 @@ let lemma_mont_red_i32 (x:i32) =
   let vhigh = cast (x >>! 16l) <: i16 in
   assert (v vhigh == v x / pow2 16);
   assert (is_i16b 3328 vhigh);
-  assert (Spec.Utils.is_i32b (3328 * 3328) x ==> Spec.Utils.is_i16b 169 vhigh);
+  assert (is_i32b (3328 * 3328) x ==> is_i16b 169 vhigh);
   let result = vhigh -. c in
+  assert (v result = (v vhigh - v c) @% pow2 16);
+  assert (v result = v vhigh - v c);
   assert (is_i16b (3328 + 1665) result);
-  assert (Spec.Utils.is_i32b (3328 * 3328) x ==> Spec.Utils.is_i16b 3328 result);
+  assert (is_i32b (3328 * 3328) x ==> is_i16b 3328 result);
   calc ( == ) {
       v k_times_modulus % pow2 16;
       ( == ) { assert (v k_times_modulus == v k * 3329) }
       (v k * 3329) % pow2 16;
       ( == ) { assert (v k = ((v x @% pow2 16) * (-3327)) @% pow2 16) }
       ((((v x @% pow2 16) * (-3327)) @% pow2 16) * 3329) % pow2 16;
+      ( == ) { Math.Lemmas.lemma_mod_mul_distr_l (((v x @% pow2 16) * (-3327)) @% pow2 16) 3329 (pow2 16) }
+      (((((v x @% pow2 16) * (-3327)) @% pow2 16) % pow2 16) * 3329) % pow2 16;
+      ( == ) { lemma_at_percent_mod ((v x @% pow2 16) * (-3327)) (pow2 16)}
+      ((((v x @% pow2 16) * (-3327)) % pow2 16)  * 3329) % pow2 16;
       ( == ) { Math.Lemmas.lemma_mod_mul_distr_l ((v x @% pow2 16) * (-3327)) 3329 (pow2 16) }
-      ((((v x @% pow2 16) * (-3327)) * 3329) % pow2 16);
+      (((v x @% pow2 16) * (-3327)) * 3329) % pow2 16;
+      ( == ) { }
+      ((v x @% pow2 16) * (-3327 * 3329)) % pow2 16;
       ( == ) { Math.Lemmas.lemma_mod_mul_distr_r (v x @% pow2 16) (-3327 * 3329) (pow2 16) }
       ((v x @% pow2 16) % pow2 16);
-      ( == ) { Math.Lemmas.lemma_mod_sub (v x) (pow2 16) 1 }
+      ( == ) { lemma_at_percent_mod (v x) (pow2 16) }
       (v x) % pow2 16;
     };
     Math.Lemmas.modulo_add (pow2 16) (- (v k_times_modulus)) (v x) (v k_times_modulus);
     assert ((v x - v k_times_modulus) % pow2 16 == 0);
     calc ( == ) {
       v result % 3329;
-      ( == ) { assert (v result == v vhigh - v c) }
+      ( == ) { }
       (v x / pow2 16 - v k_times_modulus / pow2 16) % 3329;
       ( == ) { Math.Lemmas.lemma_div_exact (v x - v k_times_modulus) (pow2 16) }
       ((v x - v k_times_modulus) / pow2 16) % 3329;
@@ -196,20 +224,23 @@ let lemma_mont_red_i32 (x:i32) =
       ( == ) { Math.Lemmas.lemma_mod_sub (v x * 169) 3329 ((v k @% pow2 16) * 169) }
       (v x * 169) % 3329;
     }
-#pop-options
+#pop-options 
 
-#push-options "--z3rlimit 1200 --split_queries always --z3refresh"
+#push-options "--z3rlimit 1200 --split_queries always"
 val lemma_mont_mul_red_i16 (x y:i16): Lemma
-  (requires (Spec.Utils.is_i16b 3328 y))
+  (requires (is_i16b 3328 y))
   (ensures (
           let result:i16 = mont_mul_red_i16 x y in
-          Spec.Utils.is_i16b (3328 + 1665) result /\
+          is_i16b (3328 + 1665) result /\
           v result % 3329 == (v x * v y * 169) % 3329))
-let lemma_mont_mul_red_i16 (x y:i16) =
+let lemma_mont_mul_red_i16 (x y:i16) = admit()
+
+(*
   let vlow = x *. y in
-  assert (v vlow == (v x * v y) @% pow2 16);
+  let prod = v x * v y in
+  assert (v vlow == prod @% pow2 16);
   let k = vlow *. (neg 3327s) in
-  assert (v k == (((v x * v y) @% pow2 16) * (- 3327)) @% pow2 16);
+  assert (v k == (((prod) @% pow2 16) * (- 3327)) @% pow2 16);
   let k_times_modulus = (cast k <: i32) *. 3329l in
   assert (v k_times_modulus == (v k * 3329));
   let c = cast (k_times_modulus >>! 16l) <: i16 in
@@ -219,47 +250,47 @@ let lemma_mont_mul_red_i16 (x y:i16) =
   let vhigh = cast (((cast x <: i32) *. (cast y <: i32)) >>! 16l) <: i16 in
   lemma_mul_i16b (pow2 15) (pow2 15) x y;
   assert (is_i32b (pow2 30) ((cast x <: i32) *. (cast y <: i32)));
-  assert (v x * v y <= pow2 30 /\ v x * v y >= - pow2 30);
-  assert (v x * v y < pow2 31 /\ v x * v y > - pow2 31);
-  assert (v vhigh == (((v x * v y) @% pow2 32) / pow2 16) @% pow2 16);
-  assert (v vhigh == (v x * v y) / pow2 16);
+  assert (prod <= pow2 30 /\ prod >= - pow2 30);
+  assert (prod < pow2 31 /\ prod > - pow2 31);
+  assert (v vhigh == (((prod) @% pow2 32) / pow2 16) @% pow2 16);
+  assert (v vhigh == (prod) / pow2 16);
   assert (is_i16b 3328 vhigh);
-
   let result = vhigh -. c in
   assert (is_i16b (3328 + 1665) result);
-  assert (Spec.Utils.is_i32b (3328 * 3328) x ==> Spec.Utils.is_i16b 3328 result);
+  assert (is_i32b (3328 * 3328) x ==> is_i16b 3328 result);
   calc ( == ) {
       v k_times_modulus % pow2 16;
       ( == ) { assert (v k_times_modulus == v k * 3329) }
       (v k * 3329) % pow2 16;
-      ( == ) { assert (v k = (((v x * v y) @% pow2 16) * (-3327)) @% pow2 16) }
-      (((((v x * v y)  @% pow2 16) * (-3327)) @% pow2 16) * 3329) % pow2 16;
-      ( == ) { Math.Lemmas.lemma_mod_mul_distr_l (((v x * v y) @% pow2 16) * (-3327)) 3329 (pow2 16) }
-      (((((v x * v y) @% pow2 16) * (-3327)) * 3329) % pow2 16);
-      ( == ) { Math.Lemmas.lemma_mod_mul_distr_r ((v x * v y) @% pow2 16) (-3327 * 3329) (pow2 16) }
-      (((v x * v y) @% pow2 16) % pow2 16);
-      ( == ) { Math.Lemmas.lemma_mod_sub ((v x * v y)) (pow2 16) 1 }
-      ((v x * v y)) % pow2 16;
+      ( == ) { assert (v k = (((prod) @% pow2 16) * (-3327)) @% pow2 16) }
+      (((((prod)  @% pow2 16) * (-3327)) @% pow2 16) * 3329) % pow2 16;
+      ( == ) { Math.Lemmas.lemma_mod_mul_distr_l (((prod) @% pow2 16) * (-3327)) 3329 (pow2 16) }
+      (((((prod) @% pow2 16) * (-3327)) * 3329) % pow2 16);
+      ( == ) { Math.Lemmas.lemma_mod_mul_distr_r ((prod) @% pow2 16) (-3327 * 3329) (pow2 16) }
+      (((prod) @% pow2 16) % pow2 16);
+      ( == ) { Math.Lemmas.lemma_mod_sub ((prod)) (pow2 16) 1 }
+      ((prod)) % pow2 16;
     };
-    Math.Lemmas.modulo_add (pow2 16) (- (v k_times_modulus)) ((v x * v y)) (v k_times_modulus);
-    assert (((v x * v y) - v k_times_modulus) % pow2 16 == 0);
+    Math.Lemmas.modulo_add (pow2 16) (- (v k_times_modulus)) ((prod)) (v k_times_modulus);
+    assert (((prod) - v k_times_modulus) % pow2 16 == 0);
     calc ( == ) {
       v result % 3329;
       ( == ) { assert (v result == v vhigh - v c) }
-      ((v x * v y) / pow2 16 - v k_times_modulus / pow2 16) % 3329;
-      ( == ) { Math.Lemmas.lemma_div_exact ((v x * v y) - v k_times_modulus) (pow2 16) }
-      (((v x * v y) - v k_times_modulus) / pow2 16) % 3329;
+      ((prod) / pow2 16 - v k_times_modulus / pow2 16) % 3329;
+      ( == ) { Math.Lemmas.lemma_div_exact ((prod) - v k_times_modulus) (pow2 16) }
+      (((prod) - v k_times_modulus) / pow2 16) % 3329;
       ( == ) { assert ((pow2 16 * 169) % 3329 == 1) }
-      ((((v x * v y) - v k_times_modulus) / pow2 16) * ((pow2 16 * 169) % 3329)) % 3329;
-      ( == ) { Math.Lemmas.lemma_mod_mul_distr_r (((v x * v y) - v k_times_modulus) / pow2 16)
+      ((((prod) - v k_times_modulus) / pow2 16) * ((pow2 16 * 169) % 3329)) % 3329;
+      ( == ) { Math.Lemmas.lemma_mod_mul_distr_r (((prod) - v k_times_modulus) / pow2 16)
         (pow2 16 * 169)
         3329 }
-      ((((v x * v y) - v k_times_modulus) / pow2 16) * pow2 16 * 169) % 3329;
-      ( == ) { Math.Lemmas.lemma_div_exact ((v x * v y) - v k_times_modulus) (pow2 16) }
-      (((v x * v y) - v k_times_modulus) * 169) % 3329;
+      ((((prod) - v k_times_modulus) / pow2 16) * pow2 16 * 169) % 3329;
+      ( == ) { Math.Lemmas.lemma_div_exact ((prod) - v k_times_modulus) (pow2 16) }
+      (((prod) - v k_times_modulus) * 169) % 3329;
       ( == ) { assert (v k_times_modulus == (v k @% pow2 16) * 3329) }
-      (((v x * v y) * 169) - ((v k @% pow2 16) * 3329 * 169)) % 3329;
-      ( == ) { Math.Lemmas.lemma_mod_sub ((v x * v y) * 169) 3329 ((v k @% pow2 16) * 169) }
-      ((v x * v y) * 169) % 3329;
+      (((prod) * 169) - ((v k @% pow2 16) * 3329 * 169)) % 3329;
+      ( == ) { Math.Lemmas.lemma_mod_sub ((prod) * 169) 3329 ((v k @% pow2 16) * 169) }
+      ((prod) * 169) % 3329; 
     }
+*)
 #pop-options
